src/Examples/Interval/CallString/Example_Interval_DG_CallString_K2.thy
@@ -275,7 +275,7 @@ text \<open>Unlike \<open>k = 1\<close>, \<open>CallFwd\<close>'s \<open>Stateme
 interpretation nest_2_routed: routed_context Sabs nest_gs nest_cfg Global2 "cs_route 2"
     "fun_of_exec_dg_st_for nest_gs (bot::ivl exec_dg_st)" "fun_of_exec_dg_st_for nest_gs cinit_ivl_st" "fun_of_exec_dg_st_for nest_gs (restrict_global_resolved_q cinit_ivl_st)"
     sigma_2 "fst nest_2_sol" "(cfg_exit nest_cfg, [])" ivl_ctx_sg_2
-    Seed2 "cs_enterc 2"
+    Seed2 "cs_context 2"
 proof (unfold_locales, goal_cases FinC SeedKey RouteAgree CallFwd CombFwd EnterAgree)
   case FinC
   show ?case by (rule nest_finC)
@@ -339,13 +339,13 @@ lemma ivl_ctx_sg_2_seed:
     and "s \<in> \<lbrakk>ivl_ctx_sg_2 (Inl (u, ctx))\<rbrakk>"
   shows "call_enter nest_gs (CallEdge dst xs es) s
            \<in> \<lbrakk>ivl_ctx_sg_2 (Inl (FunctionEntry p,
-                 cs_enterc 2 u ctx (call_enter nest_gs (CallEdge dst xs es) s)))\<rbrakk>"
+                 cs_context 2 u ctx (call_enter nest_gs (CallEdge dst xs es) s)))\<rbrakk>"
   by (rule nest_2_routed.routed_context_call[OF assms])
 
 lemma ivl_ctx_sg_2_comb:
   assumes "(cl, CallEdge dst pars args, FunctionEntry p, v) \<in> calls nest_cfg"
     and "s \<in> \<lbrakk>ivl_ctx_sg_2 (Inl (cl, c1))\<rbrakk>"
-    and "t \<in> \<lbrakk>ivl_ctx_sg_2 (Inl (FunctionResult p, cs_enterc 2 cl c1 es))\<rbrakk>"
+    and "t \<in> \<lbrakk>ivl_ctx_sg_2 (Inl (FunctionResult p, cs_context 2 cl c1 es))\<rbrakk>"
     and "call_enter_store nest_gs nest_cfg cl s es"
   shows "combine_collect nest_gs dst s t \<in> \<lbrakk>ivl_ctx_sg_2 (Inl (v, c1))\<rbrakk>"
   by (rule nest_2_routed.routed_context_comb[OF assms])
@@ -356,9 +356,9 @@ lemma cinit_le_cinit_ivl_st_2: "cinit_stores nest_gs \<subseteq> \<lbrakk>fun_of
   by (auto simp: cinit_stores_def gamma_state_def fun_of_exec_dg_st_for_def fun_of_st_cinit_ivl_st_for)
 
 theorem nest_2_activation_collect_sound:
-  "activation_collect nest_gs (admiss_exact (cs_enterc 2)) [] nest_cfg (cinit_stores nest_gs) v ctx
+  "activation_collect nest_gs (admiss_exact (cs_context 2)) [] nest_cfg (cinit_stores nest_gs) v ctx
      \<subseteq> \<lbrakk>ivl_ctx_sg_2 (Inl (v, ctx))\<rbrakk>"
-proof (rule activation_collect_sound[where sg = ivl_ctx_sg_2 and admiss = "admiss_exact (cs_enterc 2)"
+proof (rule activation_collect_sound[where sg = ivl_ctx_sg_2 and admiss = "admiss_exact (cs_context 2)"
         and startcontext = "[]"
         and S = "cinit_stores nest_gs" and g = nest_cfg and gs = nest_gs])
   \<comment> \<open>ENTRY_G\<close>
@@ -389,15 +389,15 @@ next
         \<Longrightarrow> s' \<in> \<lbrakk>ivl_ctx_sg_2 (Inl (v, c))\<rbrakk>"
     by (rule nest_2_dg.dg_ctx_act_edge)
 next
-  \<comment> \<open>ADMISS_TOTAL --- \<open>admiss_exact\<close> is total since \<open>cs_enterc 2\<close> is a function.\<close>
-  show "\<And>u c s. \<exists>c'. admiss_exact (cs_enterc 2) u c s c'"
+  \<comment> \<open>ADMISS_TOTAL --- \<open>admiss_exact\<close> is total since \<open>cs_context 2\<close> is a function.\<close>
+  show "\<And>u c s. \<exists>c'. admiss_exact (cs_context 2) u c s c'"
     by (simp add: admiss_exact_def)
 next
   \<comment> \<open>CALL --- enter routed to the truncated call string.\<close>
   fix u dst pars args p cont c s c'
   assume ce: "(u, CallEdge dst pars args, FunctionEntry p, cont) \<in> calls nest_cfg"
     and sm: "s \<in> \<lbrakk>ivl_ctx_sg_2 (Inl (u, c))\<rbrakk>"
-    and adm: "admiss_exact (cs_enterc 2) u c (call_enter nest_gs (CallEdge dst pars args) s) c'"
+    and adm: "admiss_exact (cs_context 2) u c (call_enter nest_gs (CallEdge dst pars args) s) c'"
   show "call_enter nest_gs (CallEdge dst pars args) s
           \<in> \<lbrakk>ivl_ctx_sg_2 (Inl (FunctionEntry p, c'))\<rbrakk>"
     using adm ivl_ctx_sg_2_seed[OF ce sm] by (simp add: admiss_exact_def)
@@ -406,7 +406,7 @@ next
   fix cl dst pars args p cont c1 c2 s t es
   assume ce: "(cl, CallEdge dst pars args, FunctionEntry p, cont) \<in> calls nest_cfg"
     and sm: "s \<in> \<lbrakk>ivl_ctx_sg_2 (Inl (cl, c1))\<rbrakk>"
-    and adm: "admiss_exact (cs_enterc 2) cl c1 es c2"
+    and adm: "admiss_exact (cs_context 2) cl c1 es c2"
     and tm: "t \<in> \<lbrakk>ivl_ctx_sg_2 (Inl (FunctionResult p, c2))\<rbrakk>"
     and ces: "call_enter_store nest_gs nest_cfg cl s es"
   show "combine_collect nest_gs dst s t \<in> \<lbrakk>ivl_ctx_sg_2 (Inl (cont, c1))\<rbrakk>"
